\documentclass{article}
\usepackage[imagemagick]{sagetex}

\usepackage{tikz}
\usepackage{tkz-graph}

\begin{document}
Testing.

\begin{sagesilent}
    var('x')
    Z = IntegerRing();
    m = (Z.random_element()/(x+Z.random_element())) + (Z.random_element()/(x+Z.random_element()))
    simplified = m.full_simplify()
\end{sagesilent}

Start simply with the function $m(x) = \sage{m} = \sage{simplified}$.

\begin{sagesilent}
    f = (2/(x-3)) - (3/(x+5))
    simp2 = f.full_simplify()
\end{sagesilent}

After the second sage-silent block, we have that $f(x) = \sage{f} = \sage{simp2}$.

\end{document}
%sagemathcloud={"zoom_width":155}